\section{$Z$-Transform of Downsampled Signals}\label{sec:p6}

Let
\[p_N[n] = \begin{cases}
1, & n = mN\\ 0, & \text{else}
\end{cases}\]
\begin{align*}
	\Rightarrow P_N(z)
	= \sum_{n \in \mathbb{Z}} p_N[n] z^{-n} 
	= \sum_{n \in \mathbb{Z}} z^{-Nn} 
	= \sum_{n \in \mathbb{Z}} W^{-n}
\end{align*}
We have
\[\frac{1}{N} \sum_{k=0}^{N-1} W^{nk} = \begin{cases}
\frac{1}{N} \times N = 1, & n = mN\\
0, & \text{else}
\end{cases} = p_N[n]\]
Therefore
\begin{align*}
	Y(z)
	&= \sum_{n \in \mathbb{Z}} y[n] z^{-n} \\
	&= \sum_{n \in \mathbb{Z}} x[Nn] z^{-n} \\
	&= \sum_{k = Nn, n \in \mathbb{Z}} x[k] z^{-k/N} \\
	&= \sum_{k \in \mathbb{Z}} x[k] z^{-k/N} p_N[k] \\
	&= \frac{1}{N} \sum_{m=0}^{N-1} \sum_{k \in \mathbb{Z}} W^{mk} z^{-k/N} x[k] \\
	&= \frac{1}{N} \sum_{m=0}^{N-1}X(W^m z^{1/N})
\end{align*}
Replacing $z$ with $e^{j\omega}$, we have
