\section{Lagrange Interpolation}\label{sec:p2}

\begin{enumerate}[(a)]
\item We have 
\[p_{\tilde{D}}(t) = p_D(t) + c(t-t_0)(t-t_1)\cdots(t-t_{N-1}) = p_D(t) = p_D(t) + c\prod_{j=0}^{N-1}(t-t_j)\]
We want $p_{\tilde{D}}(t_N) = x_N$, so
\[c\prod_{j=0}^{N-1}(t-t_j) = x_N \Leftrightarrow c = \frac{x_N}{\prod_{j=0}^{N-1}(t_N-t_j)}\]

\item We already have
\begin{align*}
	p_{\tilde{D}}(t)
	&= p_D(t) + \frac{x_N}{\prod_{j=0}^{N-1}(t_N-t_j)} \prod_{j=0}^{N-1}(t-t_j) \\
	&= p_D(t) + x_N \prod_{j=0}^{N-1}\frac{t-t_j}{t_N-t_j} \\
	&= p_{D^{(-1)}}(t) + x_{N-1} \prod_{j=0}^{N-2}\frac{t-t_j}{t_{N-1}-t_j} + x_N \prod_{j=0}^{N-1}\frac{t-t_j}{t_N-t_j} \\
\end{align*}
where $D^{(-1)} = D / \{(t_{N-1}m x_{N-1})\} = \{(t_k,x_k)\}_{k=0}^{N-2}$. Therefore, in general
\[p_{\tilde{D}}(t) = \sum_{k=0}^{N}x_k \prod_{j \neq k}\frac{t-t_j}{t_k-t_j}  \]
\[\Rightarrow p_{D}(t) = \sum_{k=0}^{N-1}x_k \prod_{j \neq k}\frac{t-t_j}{t_k-t_j}\]

\end{enumerate}