\section{Some basic properties of inner product spaces}\label{sec:part2}
Notice that:
\[\innerprod{a}{b+c}  = \overline{\innerprod{b+c}{a}} = \overline{\innerprod{b}{a}} + \overline{\innerprod{c}{a}} = \innerprod{a}{b} + \innerprod{a}{c}.\]

\subsection{The Cauchy-Schwarz inequality}
\[\abs{\innerprod{x}{y}} \leq \norm{x} \norm{y}\]
\begin{proof}
	If $\innerprod{x}{y} = 0$, then theorem holds because $\norm{x}$ and $\norm{y} \geq 0.$
	
	Suppose that $x \neq 0$ and $y \neq 0$. Let $z \in \mathbb{C}$, such that:
	\[z = \frac{\innerprod{x}{y}}{\norm{y}^2} = \frac{\overline{\innerprod{y}{x}}}{\norm{y}^2}.\]
	
	We have
	\begin{align*}
		0 &\leq \norm{x - zy}^2 = \innerprod{x-zy}{x-zy} = \innerprod{x}{x-zy} - \innerprod{zy}{x-zy} \\
		&= \innerprod{x}{x} - \innerprod{x}{zy} - \innerprod{zy}{x} + \innerprod{zy}{zy} \\
		&= \norm{x}^2 -\bar{z}\innerprod{x}{y} - z\innerprod{y}{x} + z \bar{z} \norm{y}^2 \\
		&= \norm{x}^2 - \frac{\innerprod{y}{x}\innerprod{x}{y}}{\norm{y}^2} - \frac{\innerprod{x}{y}\innerprod{y}{x}}{\norm{y}^2} + \frac{\innerprod{x}{y}}{\norm{y}^2} \frac{\innerprod{y}{x}}{\norm{y}^2} \norm{y}^2 \\
		&= \norm{x}^2 - \frac{\innerprod{x}{y}\innerprod{y}{x}}{\norm{y}^2} \\
		&= \norm{x}^2 - \frac{\abs{\innerprod{x}{y}}^2}{\norm{y}^2}.
	\end{align*}
	Therefore,
	\begin{align*}
		&0 \leq \norm{x}^2 - \frac{\abs{\innerprod{x}{y}}^2}{\norm{y}^2} \\
		\Leftrightarrow & \norm{x}^2 \geq \frac{\abs{\innerprod{x}{y}}^2}{\norm{y}^2} \\
		\Leftrightarrow & \norm{x}^2 \norm{y}^2 \geq \abs{\innerprod{x}{y}}^2 \\
		\Leftrightarrow & \norm{x} \norm{y} \geq \abs{\innerprod{x}{y}}.
	\end{align*}
\end{proof}

The equality occurs iff $x = \alpha y$, for some scalar $\alpha$.
\begin{proof}
	By substituting $x = \alpha y$, we have
	\[\abs{\innerprod{x}{y}} = \abs{\innerprod{\alpha y}{y}} = \abs{x} \abs{\innerprod{y}{y}} = \abs{\alpha} \norm{y}^2 = \abs{\alpha} \norm{y} \norm{y} = \norm{x} \norm{y}.\]
\end{proof}

\subsection{The triangle inequality}
$\norm{x + y}^2 \leq \norm{x} + \norm{y}$ with equality iff $y = \alpha x$
\begin{proof}
	\begin{align*}
		\norm{x + y}^2 &= \innerprod{x+y}{x+y} \\
		&= \innerprod{x}{x+y} + \innerprod{y}{x+y}\\
		&= \innerprod{x}{x} + \innerprod{x}{y} + \innerprod{y}{x} + \innerprod{y}{y} \\
		&= \norm{x}^2 + \norm{y}^2 + \innerprod{x}{y} + \innerprod{y}{x}
	\end{align*}
	
	By Cauchy-Schwarz inequality:
	\begin{align*}
		& \innerprod{x}{y} \leq \norm{x} \norm{y}\\
		\Rightarrow & \innerprod{y}{x} \leq \norm{x} \norm{y}\\
		\Rightarrow & \innerprod{x}{y} + \innerprod{y}{x} \leq 2\norm{x}\norm{y}.
	\end{align*}
	
	Therefore,
	\begin{align*}
		&\norm{x + y}^2 \leq \norm{x} + \norm{y}^2 + 2\norm{x}\norm{y} = (\norm{x} + \norm{y})^2 \\
		\Rightarrow & \norm{x + y} \leq \norm{x} + \norm{y} \qquad \because \text{norms are non-negative.}
	\end{align*}
	
	If $y = \alpha x$ then the equality of Cauchy-Schwarz theorem occurs. Therefore,
	\begin{align*}
		&\innerprod{x}{y} + \innerprod{y}{x} = 2 \norm{x} \norm{y} \\
		\Rightarrow &\norm{x + y}^2 = \norm{x}^2 + \norm{y}^2 + 2 \norm{x} \norm{y} = (\norm{x} + \norm{y})^2 \\
		\Rightarrow & \norm{x + y} = \norm{x} + \norm{y}.
	\end{align*}
\end{proof}


\subsection{Parallelogram law}
\[\norm{x+y}^2 + \norm{x-y}^2 = 2(\norm{x}^2 + \norm{y}^2)\]

\begin{proof}
	\begin{align*}
		LHS &= \innerprod{x+y}{x+y} + \innerprod{x-y}{x-y} \\
		&= (\norm{x}^2 + \norm{y}^2 + \innerprod{x}{y} + \innerprod{y}{x}) + (\norm{x}^2 + \norm{y}^2 - \innerprod{x}{y} - \innerprod{y}{x}) \\
		&= 2(\norm{x}^2 + \norm{y}^2) = RHS.
	\end{align*}
\end{proof}